Examples/Kruskal/UGraph_Impl.thy
@@ -1,0 +1,235 @@
+theory UGraph_Impl
+imports
+ Kruskal_Impl "../../../Kruskal/UGraph" "SepLogicTime_RBTreeBasic.Asymptotics_2D" 
+begin
+
+abbreviation "subforest' EE F \<equiv> forest F \<and> F \<subseteq> EE"
+
+definition "spanningforest' EE F \<longleftrightarrow> subforest' EE F \<and> (\<forall>x \<in> EE - F. \<not> subforest' EE (insert x F))"
+
+definition "MST' EE w F \<longleftrightarrow> spanningforest' EE F \<and> (\<forall>F'. spanningforest' EE F' \<longrightarrow> sum w F \<le> sum w F')"
+
+ 
+
+locale uGraph_impl = uGraph E w for E :: "nat uprod set" and w :: "nat uprod \<Rightarrow> int" +
+  fixes getEdges_impl :: "(nat \<times> int \<times> nat) list Heap"
+    and getEdges_time sort_time :: nat
+    and empty_uf_time indep_test_time insert_uf_time :: nat
+  assumes getEdges_impl[sepref_fr_rules]:
+    "(uncurry0 getEdges_impl,  uncurry0 (PR_CONST (SPECT (emb (\<lambda>L. lst_graph_P' w L E) getEdges_time)))) \<in> unit_assn\<^sup>k \<rightarrow>\<^sub>a list_assn (nat_assn \<times>\<^sub>a int_assn \<times>\<^sub>a nat_assn)"
+   
+begin
+
+
+abbreviation "subforest EE F \<equiv> forest F \<and> F \<subseteq> EE"
+
+sublocale  Kruskal_intermediate_Impl0 E "subforest E" "uconnectedV" "epath" w 
+    "PR_CONST (SPECT (emb (\<lambda>L. lst_graph_P' w L E) getEdges_time))" getEdges_impl
+    getEdges_time sort_time
+    empty_uf_time indep_test_time insert_uf_time
+proof (unfold_locales, goal_cases)
+  fix e
+  assume "e\<in>E"
+  then show "proper_uprod e" using ecard2 by auto
+next
+  show "finite E" by simp
+next
+  fix E'
+  assume "forest E' \<and> E' \<subseteq> E"
+  then show "E' \<subseteq> E" by auto
+next
+  show "forest {} \<and> {} \<subseteq> E" apply (auto simp: decycle_def forest_def)
+    using epath.elims(2) by fastforce 
+next
+  fix X Y
+  assume "forest X \<and> X \<subseteq> E" "Y \<subseteq> X" 
+  then show "forest Y \<and> Y \<subseteq> E" using forest_mono by auto
+next
+  fix u v E'
+  show " ((u, v) \<in> uconnectedV E') = (\<exists>p. epath E' u p v \<and> u \<in> Kruskal_intermediate_defs.V E \<and> v \<in> Kruskal_intermediate_defs.V E)"
+    unfolding uconnected_def Kruskal_intermediate_defs.V_def by auto
+next
+  case (7 u v)
+  then show ?case unfolding uconnected_def Kruskal_intermediate_defs.V_def apply auto 
+    using epath.elims(2) by force 
+next
+  case (8 E1 u p v E2)
+  then have "\<exists>a b. (a, b) \<notin> uconnected E2
+           \<and> Upair a b \<notin> E2 \<and> Upair a b \<in> E1" by(rule findaugmenting_edge)
+  then show ?case by auto
+next
+  fix F u v
+  assume f: "forest F \<and> F \<subseteq> E" and notin: "Upair u v \<in> E - F"
+  from notin ecard2 have unv: "u\<noteq>v" by fastforce
+  show "(forest (insert (Upair u v) F) \<and> insert (Upair u v) F \<subseteq> E) = ((u, v) \<notin> uconnectedV F)"
+  proof
+    assume a: "forest (insert (Upair u v) F) \<and> insert (Upair u v) F \<subseteq> E "
+    have "(u, v) \<notin> uconnected F" apply(rule insert_stays_forest_means_not_connected)
+      using notin a unv by auto
+    then show "((u, v) \<notin> Restr (uconnected F) (UNION E set_uprod))" by auto
+  next 
+    assume a: "(u, v) \<notin> Restr (uconnected F) (UNION E set_uprod)"
+    have "forest (insert (Upair u v) F)" apply(rule augment_forest_overedges[where E=E])
+      using notin f a unv  by auto 
+    moreover have "insert (Upair u v) F \<subseteq> E"
+      using notin f by auto
+    ultimately show "forest (insert (Upair u v) F) \<and> insert (Upair u v) F \<subseteq> E" by auto
+  qed
+next      
+  fix F
+  assume "F\<subseteq>E"
+  show "equiv (Kruskal_intermediate_defs.V E) (uconnectedV F)"
+    unfolding  Kruskal_intermediate_defs.V_def by(rule equiv_vert_uconnected)
+next                                 
+  case (11 F)
+  then show ?case unfolding  Kruskal_intermediate_defs.V_def by auto
+next
+  case (12 x y F)
+  then show ?case unfolding  Kruskal_intermediate_defs.V_def by (rule insert_uconnectedV_per)
+next
+  show "E \<noteq> {}" by simp
+  show "PR_CONST (getEdges' w E (enat getEdges_time)) \<le> \<Down> Id (getEdges' w E (enat getEdges_time))" using  PR_CONST_def by simp
+  show "(uncurry0 getEdges_impl, uncurry0 (PR_CONST (getEdges' w E (enat getEdges_time)))) \<in> unit_assn\<^sup>k \<rightarrow>\<^sub>a list_assn (nat_assn \<times>\<^sub>a int_assn \<times>\<^sub>a nat_assn)"
+    using getEdges_impl by simp
+qed
+ 
+lemma minBasis_is_MST': "minBasis = MST' E w"
+  unfolding minBasis_def MST'_def
+   basis_def  spanningforest'_def by simp
+
+end
+
+
+locale uGraph_impl2 = uGraph_impl + UnionFind_Impl + sortMaxnode +
+  assumes 
+  [simp]:  "uf_init_time (Suc (Max V)) \<le> empty_uf_time" 
+    "uf_cmp_time (Suc (Max V)) \<le> indep_test_time" 
+    "uf_union_time (Suc (Max V)) \<le> insert_uf_time" 
+    "sort_time' (card E) \<le> sort_time"
+begin
+ 
+
+sublocale s: Kruskal_intermediate_Impl E "subforest E" "uconnectedV" "epath" w "PR_CONST getEdges" getEdges_impl
+  getEdges_time sort_time empty_uf_time indep_test_time insert_uf_time is_uf
+     uf_init uf_init_time uf_cmp uf_cmp_time uf_union uf_union_time sortEdges_impl sort_time'
+  apply (unfold_locales)
+        apply simp apply simp
+  subgoal  using getEdges_impl PR_CONST_def by auto
+     apply simp_all
+  done
+
+term MST
+
+lemmas kurskal_horetriple =  s.kruskal_correct_forest
+thm s.kruskal_ref_spec
+abbreviation "kruskal \<equiv> s.kruskal"
+
+end
+
+thm uGraph_impl2.kurskal_horetriple
+thm uGraph_impl2_def
+(*
+definition getEdges_time :: "nat \<Rightarrow>  nat" where "getEdges_time = undefined"
+definition sort_time' :: "nat \<Rightarrow>  nat" where "sort_time' = undefined"
+definition uf_init_time :: "nat \<Rightarrow>  nat" where "uf_init_time = undefined"
+definition uf_cmp_time :: "nat \<Rightarrow>  nat" where "uf_cmp_time = undefined"
+definition uf_union_time :: "nat \<Rightarrow>  nat" where "uf_union_time = undefined"
+lemma [asym_bound]: "getEdges_time \<in> \<Theta>(\<lambda>n::nat. n)" sorry
+  lemma [asym_bound]: "sort_time' \<in> \<Theta>(\<lambda>n::nat. n * ln n)" sorry
+  lemma [asym_bound]: "uf_init_time \<in> \<Theta>(\<lambda>n::nat. 1)" sorry
+  lemma [asym_bound]: "uf_cmp_time \<in> \<Theta>(\<lambda>n::nat. 1)" sorry
+  lemma [asym_bound]: "uf_union_time \<in> \<Theta>(\<lambda>n::nat. ln n)" sorry
+ 
+
+
+fun kruskal_time :: "nat * nat \<Rightarrow> nat" where "kruskal_time (sE, mV) = 
+      (getEdges_time sE + sort_time' sE + (12 + uf_init_time mV) +
+      sE * (uf_cmp_time mV + (23 + uf_union_time mV)))"
+
+term "\<Theta>\<^sub>2(\<lambda>(e::nat,m::nat). e * ln e + e * ln m + e )"
+                                                                  
+lemma "kruskal_time \<in> \<Theta>\<^sub>2(\<lambda>(e::nat,m::nat). e * ln e + e * ln m  )"
+  apply (subst surjective_pairing)
+  unfolding kruskal_time.simps
+  by auto2
+
+
+locale krtime = fixes
+  getEdges_time :: "nat \<Rightarrow>  nat"  
+ and sort_time' :: "nat \<Rightarrow>  nat"  
+and uf_init_time :: "nat \<Rightarrow>  nat"  
+and uf_cmp_time :: "nat \<Rightarrow>  nat"  
+and uf_union_time :: "nat \<Rightarrow>  nat"  
+assumes [asym_bound]: "getEdges_time \<in> \<Theta>(\<lambda>n::nat. n)"  
+  and [asym_bound]: "sort_time' \<in> \<Theta>(\<lambda>n::nat. n * ln n)" 
+  and [asym_bound]: "uf_init_time \<in> \<Theta>(\<lambda>n::nat. 1)" 
+  and [asym_bound]: "uf_cmp_time \<in> \<Theta>(\<lambda>n::nat. 1)" 
+  and [asym_bound]: "uf_union_time \<in> \<Theta>(\<lambda>n::nat. ln n)" 
+begin
+
+
+fun kruskal_time :: "nat * nat \<Rightarrow> nat" where "kruskal_time (sE, mV) = 
+      (getEdges_time sE + sort_time' sE + (12 + uf_init_time mV) +
+      sE * (uf_cmp_time mV + (23 + uf_union_time mV)))"
+
+                                                                  
+lemma "kruskal_time \<in> \<Theta>\<^sub>2(\<lambda>(e::nat,m::nat). e * ln e + e * ln m  )"
+  apply (subst surjective_pairing)
+  unfolding kruskal_time.simps
+  by auto2
+
+end
+*)
+
+locale stuffdone = UnionFind_Impl + sortMaxnode
+  + fixes "getEdges_time" :: "nat \<Rightarrow> nat"
+  assumes
+      [asym_bound]: "getEdges_time \<in> \<Theta>(\<lambda>n::nat. n)" 
+  and [asym_bound]: "sort_time' \<in> \<Theta>(\<lambda>n::nat. n * ln n)" 
+  and [asym_bound]: "uf_init_time \<in> \<Theta>(\<lambda>n::nat. 1)" 
+  and [asym_bound]: "uf_cmp_time \<in> \<Theta>(\<lambda>n::nat. 1)" 
+  and [asym_bound]: "uf_union_time \<in> \<Theta>(\<lambda>n::nat. ln n)" 
+begin
+
+
+fun kruskal_time :: "nat * nat \<Rightarrow> nat" where "kruskal_time (sE, mV) = 
+      (getEdges_time sE + sort_time' sE + (12 + uf_init_time mV) +
+      sE * (uf_cmp_time mV + (23 + uf_union_time mV)))"
+
+term "\<Theta>\<^sub>2(\<lambda>(e::nat,m::nat). e * ln e + e * ln m + e )"
+                                                                  
+lemma "kruskal_time \<in> \<Theta>\<^sub>2(\<lambda>(e::nat,m::nat). e * ln e + e * ln m   )"
+  apply (subst surjective_pairing)
+  unfolding kruskal_time.simps
+  apply (auto2) sorry
+
+lemma 
+  assumes [simp]: "\<And>e. e \<in> E \<Longrightarrow> proper_uprod e" "finite E" "E \<noteq> {}"
+      and getEdges_impl:
+    "(uncurry0 getEdges_impl,  uncurry0 (PR_CONST (SPECT (emb (\<lambda>L. lst_graph_P' w L E) (enat (getEdges_time (card E))))))) \<in> unit_assn\<^sup>k \<rightarrow>\<^sub>a list_assn (nat_assn \<times>\<^sub>a int_assn \<times>\<^sub>a nat_assn)"
+   
+  shows "<$ (kruskal_time (card E,Suc (Max (uGraph.verts E))) )>
+             uGraph_impl2.kruskal getEdges_impl uf_init uf_cmp uf_union sortEdges_impl
+         <\<lambda>r. \<exists>\<^sub>Ara. hr_comp (da_assn id_assn) (lst_graph_rel' w) ra r * \<up> ( MST' E w ra)>\<^sub>t"
+proof -
+
+  interpret uGraph_impl2 E w  getEdges_impl 
+      "getEdges_time (card E)" "sort_time' (card E)"   "uf_init_time (Suc (Max (uGraph.verts E)))"
+        "uf_cmp_time (Suc (Max (uGraph.verts E)))" "uf_union_time (Suc (Max (uGraph.verts E)))"
+  is_uf   uf_init  uf_init_time uf_cmp  uf_cmp_time  uf_union  uf_union_time  sortEdges_impl  sort_time'  
+    apply unfold_locales
+       apply (simp_all add: Kruskal_intermediate_defs.V_def)
+    using getEdges_impl    
+    by auto
+
+  from kurskal_horetriple show ?thesis
+    unfolding minBasis_time_def minBasis_is_MST' kruskal_time.simps .
+qed
+  
+
+
+end
+
+
+
+end
